Add lists; greatly improve progress proof/formulation

formalization/Psamathe.thy
@@ -3,14 +3,17 @@ theory Psamathe
 begin
 
 datatype TyQuant = empty | any | one | nonempty
-datatype BaseTy = natural | boolean
+datatype BaseTy = natural | boolean 
+  | table "string list" "TyQuant \<times> BaseTy"
 type_synonym Type = "TyQuant \<times> BaseTy"
 datatype Mode = s | d
 datatype SVal = SLoc nat | Amount nat
 type_synonym StorageLoc = "nat \<times> SVal" 
 datatype Stored = V string | Loc StorageLoc
 datatype Locator = N nat | B bool | S Stored
-                 | VDef string BaseTy ("var _ : _")
+  | VDef string BaseTy ("var _ : _")
+  | EmptyList Type ("[ _ ; ]")
+  | ConsList Type "Locator" "Locator" ("[ _ ; _ , _ ]")
 datatype Stmt = Flow Locator Locator
 datatype Prog = Prog "Stmt list"
 
@@ -18,30 +21,6 @@ type_synonym Env = "(Stored, Type) map"
 
 definition toQuant :: "nat \<Rightarrow> TyQuant" where
   "toQuant n \<equiv> (if n = 0 then empty else if n = 1 then one else nonempty)"
-
-inductive loc_type :: "Env \<Rightarrow> Mode \<Rightarrow> Locator \<Rightarrow> Type \<Rightarrow> (Type \<Rightarrow> Type) \<Rightarrow> Env \<Rightarrow> bool"
-  ("_ \<turnstile>{_} _ : _ ; _ \<stileturn> _") where
-  Nat: "\<Gamma> \<turnstile>{s} (N n) : (toQuant(n), natural) ; f \<stileturn> \<Gamma>"
-| Bool: "\<Gamma> \<turnstile>{s} (B b) : (one, boolean) ; f \<stileturn> \<Gamma>"
-| Var: "\<lbrakk> \<Gamma> x = Some \<tau> \<rbrakk> \<Longrightarrow> \<Gamma> \<turnstile>{m} (S x) : \<tau> ; f \<stileturn> (\<Gamma>(x \<mapsto> f(\<tau>)))"
-| VarDef: "\<lbrakk> V x \<notin> dom \<Gamma> \<rbrakk> \<Longrightarrow> \<Gamma> \<turnstile>{d} (var x : t) : (empty, t) ; f \<stileturn> (\<Gamma>(V x \<mapsto> f(empty, t)))"
-
-datatype Val = Num nat | Bool bool | error
-type_synonym Resource = "BaseTy \<times> Val"
-type_synonym Store = "(string, StorageLoc) map \<times> (nat, Resource) map"
-
-fun emptyVal :: "BaseTy \<Rightarrow> Val" where
-  "emptyVal natural = Num 0"
-| "emptyVal boolean = Bool False"
-
-inductive loc_eval :: "Store \<Rightarrow> Locator \<Rightarrow> Store \<Rightarrow> Locator \<Rightarrow> bool"
-  ("< _ , _ > \<rightarrow> < _ , _ >") where
-  ENat: "\<lbrakk> l \<notin> dom \<rho> \<rbrakk> \<Longrightarrow> < (\<mu>, \<rho>), N n > \<rightarrow> < (\<mu>, \<rho>(l \<mapsto> (natural, Num n))), S (Loc (l, Amount n)) >"
-| EBool: "\<lbrakk> l \<notin> dom \<rho> \<rbrakk> \<Longrightarrow> < (\<mu>, \<rho>), B b > \<rightarrow> < (\<mu>, \<rho>(l \<mapsto> (boolean, Bool b))), S (Loc (l, SLoc l)) >"
-| EVar: "\<lbrakk> \<mu> x = Some l \<rbrakk> \<Longrightarrow> < (\<mu>, \<rho>), S (V x) > \<rightarrow> < (\<mu>, \<rho>), S (Loc l) >"
-| EVarDef: "\<lbrakk> x \<notin> dom \<mu> ; l \<notin> dom \<rho> \<rbrakk> 
-            \<Longrightarrow> < (\<mu>, \<rho>), var x : t > 
-                \<rightarrow> < (\<mu>(x \<mapsto> (l, SLoc l)), \<rho>(l \<mapsto> (t, emptyVal t))), S (Loc (l, SLoc l)) >"
 
 fun addQuant :: "TyQuant \<Rightarrow> TyQuant \<Rightarrow> TyQuant" ("_ \<oplus> _") where
   "(q \<oplus> empty) = q"
@@ -52,52 +31,182 @@ fun addQuant :: "TyQuant \<Rightarrow> TyQuant \<Rightarrow> TyQuant" ("_ \<oplu
 | "(r \<oplus> one) = nonempty"
 | "(any \<oplus> any) = any"
 
+inductive loc_type :: "Env \<Rightarrow> Mode \<Rightarrow> Locator \<Rightarrow> Type \<Rightarrow> (Type \<Rightarrow> Type) \<Rightarrow> Env \<Rightarrow> bool"
+  ("_ \<turnstile>{_} _ : _ ; _ \<stileturn> _") where
+  Nat: "\<Gamma> \<turnstile>{s} (N n) : (toQuant(n), natural) ; f \<stileturn> \<Gamma>"
+| Bool: "\<Gamma> \<turnstile>{s} (B b) : (one, boolean) ; f \<stileturn> \<Gamma>"
+| Var: "\<lbrakk> \<Gamma> x = Some \<tau> \<rbrakk> \<Longrightarrow> \<Gamma> \<turnstile>{m} (S x) : \<tau> ; f \<stileturn> (\<Gamma>(x \<mapsto> f(\<tau>)))"
+| VarDef: "\<lbrakk> V x \<notin> dom \<Gamma> \<rbrakk> \<Longrightarrow> \<Gamma> \<turnstile>{d} (var x : t) : (empty, t) ; f \<stileturn> (\<Gamma>(V x \<mapsto> f(empty, t)))"
+| EmptyList: "\<Gamma> \<turnstile>{s} [ \<tau> ; ] : (empty, table [] \<tau>) ; f \<stileturn> \<Gamma>"
+| ConsList: "\<lbrakk> \<Gamma> \<turnstile>{s} \<L> : \<tau> ; f \<stileturn> \<Delta> ;
+              \<Delta> \<turnstile>{s} Tail : (q, table [] \<tau>) ; f \<stileturn> \<Xi> \<rbrakk> 
+             \<Longrightarrow> \<Gamma> \<turnstile>{s} [ \<tau> ; \<L>, Tail ] : (one \<oplus> q, table [] \<tau>) ; f \<stileturn> \<Xi>"
+
+datatype Val = Num nat | Bool bool 
+  | Table "StorageLoc list"
+  | error
+type_synonym Resource = "BaseTy \<times> Val"
+type_synonym Store = "(string, StorageLoc) map \<times> (nat, Resource) map"
+
+fun emptyVal :: "BaseTy \<Rightarrow> Val" where
+  "emptyVal natural = Num 0"
+| "emptyVal boolean = Bool False"
+| "emptyVal (table keys t) = Table []"
+
+fun located :: "Locator \<Rightarrow> bool" where
+  "located (S (Loc _)) = True"
+| "located [ \<tau> ; ] = True"
+| "located [ \<tau> ; Head, Tail ] = (located Head \<and> located Tail)"
+| "located _ = False"
+
+inductive loc_eval :: "Store \<Rightarrow> Locator \<Rightarrow> Store \<Rightarrow> Locator \<Rightarrow> bool"
+  ("< _ , _ > \<rightarrow> < _ , _ >") where
+  ENat: "\<lbrakk> l \<notin> dom \<rho> \<rbrakk> \<Longrightarrow> < (\<mu>, \<rho>), N n > \<rightarrow> < (\<mu>, \<rho>(l \<mapsto> (natural, Num n))), S (Loc (l, Amount n)) >"
+| EBool: "\<lbrakk> l \<notin> dom \<rho> \<rbrakk> \<Longrightarrow> < (\<mu>, \<rho>), B b > \<rightarrow> < (\<mu>, \<rho>(l \<mapsto> (boolean, Bool b))), S (Loc (l, SLoc l)) >"
+| EVar: "\<lbrakk> \<mu> x = Some l \<rbrakk> \<Longrightarrow> < (\<mu>, \<rho>), S (V x) > \<rightarrow> < (\<mu>, \<rho>), S (Loc l) >"
+| EVarDef: "\<lbrakk> x \<notin> dom \<mu> ; l \<notin> dom \<rho> \<rbrakk> 
+            \<Longrightarrow> < (\<mu>, \<rho>), var x : t > 
+                \<rightarrow> < (\<mu>(x \<mapsto> (l, SLoc l)), \<rho>(l \<mapsto> (t, emptyVal t))), S (Loc (l, SLoc l)) >"
+| EConsListHeadCongr: "\<lbrakk> < \<Sigma>, \<L> > \<rightarrow> < \<Sigma>', \<L>' > \<rbrakk>
+                   \<Longrightarrow> < \<Sigma>, [ \<tau> ; \<L>, Tail ] > \<rightarrow> < \<Sigma>', [ \<tau> ; \<L>', Tail ] >"
+| EConsListTailCongr: "\<lbrakk> located \<L> ; < \<Sigma>, Tail > \<rightarrow> < \<Sigma>', Tail' > \<rbrakk>
+              \<Longrightarrow> < \<Sigma>, [ \<tau> ; \<L>, Tail ] > \<rightarrow> < \<Sigma>', [ \<tau> ; \<L>, Tail' ] >"
+
+(* TODO: Should replace direct lookup by select, probably. Actually, this rule isn't needed, I think, 
+  because we only need to allocate the list if we are flowing from it.
+| EConsList: "\<lbrakk> \<rho> tailLoc = Some (table [] \<tau>, Table locs) \<rbrakk>
+              \<Longrightarrow> < (\<mu>, \<rho>), [ \<tau> ; S (Loc l), S (Loc (tailLoc, SLoc tailLoc)) ] > 
+                  \<rightarrow> < (\<mu>, \<rho>(tailLoc \<mapsto> (table [] \<tau>, Table (l # locs)))), S (Loc (tailLoc, SLoc tailLoc)) >"
+*)
+(* | EEmptyList: "\<lbrakk> l \<notin> dom \<rho> \<rbrakk>
+               \<Longrightarrow> < (\<mu>, \<rho>), [ \<tau> ; ] > \<rightarrow> < (\<mu>, \<rho>(l \<mapsto> (table [] \<tau>, Table []))), S (Loc (l, SLoc l)) >"
+*)
+
 definition var_dom :: "Env \<Rightarrow> string set" where
   "var_dom \<Gamma> \<equiv> { x . V x \<in> dom \<Gamma> }"
 
+(* This is a weaker version of compatibility (tentatively, locator compatibility)
+  This is needed, because while evaluating locators, the type environments won't agree with the 
+  actual state of the store (TODO: Could resolve this by going to old updater system),
+  because the type environment represents the state of the store *after* the flow occurs. 
+  So we will need some separate "statement compatibility" definition, which includes stronger
+  conditions on the state of the store (e.g., type quantities being correct, the only strengthening
+  I think we will need)*)
 fun compat :: "Env \<Rightarrow> Store \<Rightarrow> bool" ("_ \<leftrightarrow> _") where
   "compat \<Gamma> (\<mu>, \<rho>) = ((var_dom \<Gamma> = dom \<mu>) \<and> 
-                      (\<forall>x l k. \<mu> x = Some (l, k) \<longrightarrow> \<rho> l \<noteq> None))"
-                      (* (\<forall>x q t. \<Gamma>(V x) = Some (q,t) \<longrightarrow> (\<exists>l v. \<rho> l = Some (t, v))))" *)
+                      (\<forall>x l k. \<mu> x = Some (l, k) \<longrightarrow> \<rho> l \<noteq> None) \<and>
+                      (\<forall>x q t. \<Gamma>(V x) = Some (q,t) \<longrightarrow> (\<exists>l v. \<rho> l = Some (t, v))))" 
 
-definition located :: "Locator \<Rightarrow> bool" where
-  "located \<L> \<equiv> case \<L> of S (Loc _) \<Rightarrow> True | _ \<Rightarrow> False"
-
-lemma locator_progress:
-  fixes "\<Gamma>" and "\<L>" and "\<tau>" and "\<Delta>" and "\<mu>" and "\<rho>" and "l"
-  assumes "\<Gamma> \<turnstile>{s} \<L> : \<tau> ; (\<lambda>(_, t'). (empty, t')) \<stileturn> \<Delta>"
-      and "\<Gamma> \<leftrightarrow> (\<mu>, \<rho>)"
-      and "l \<notin> dom \<rho>" (* For convenience only *)
-   shows "located \<L> \<or> (\<exists>\<mu>' \<rho>' \<L>'. (\<Delta> \<leftrightarrow> (\<mu>', \<rho>')) \<and> < (\<mu>, \<rho>), \<L> > \<rightarrow> < (\<mu>', \<rho>'), \<L>' >)"
+(* Might not work. 
+The type rule gives the type environment after the entire thing has been evaluated, not one step...
+lemma compat_progress:
+  fixes "\<Gamma>" and "\<L>" and "\<tau>" and "\<Delta>" and "\<Sigma>" and "\<Sigma>'" and "\<L>'" and "m"
+  assumes "< \<Sigma>, \<L> > \<rightarrow> < \<Sigma>', \<L>' >"
+      and "\<Gamma> \<turnstile>{m} \<L> : \<tau> ; f \<stileturn> \<Delta>"
+      and "\<Gamma> \<leftrightarrow> \<Sigma>"
+    shows "\<Delta> \<leftrightarrow> \<Sigma>'"
   using assms
-proof(induction rule: loc_type.induct)
+proof(induction arbitrary: \<Gamma> \<Delta> \<tau> f m rule: loc_eval.induct)
+  case (ENat l \<rho> \<mu> n)
+  then show ?case
+(* TODO: Why do I have to write it like this? *)
+    by simp (erule loc_type.cases, auto)
+next
+  case (EBool l \<rho> \<mu> b)
+  then show ?case
+    by simp (erule loc_type.cases, auto)
+next
+  case (EVar \<mu> x l \<rho>)
+  then show ?case 
+    by simp (erule loc_type.cases, auto simp: var_dom_def)
+next
+  case (EVarDef x \<mu> l \<rho> t)
+  then show ?case
+    by simp (erule loc_type.cases, auto simp: var_dom_def)
+next
+  case (EConsListHeadCongr \<Sigma> \<L> \<Sigma>' \<L>' \<tau>' Tail)
+  then have eval: "< \<Sigma> , \<L> > \<rightarrow> < \<Sigma>' , \<L>' >"
+    and induct: "\<And>\<Gamma>' \<Delta>' m \<sigma> g. \<lbrakk>\<Gamma>' \<turnstile>{m} \<L> : \<sigma> ; g \<stileturn> \<Delta>'; \<Gamma>' \<leftrightarrow> \<Sigma>\<rbrakk> \<Longrightarrow> \<Delta>' \<leftrightarrow> \<Sigma>'"
+    and typed: "\<Gamma> \<turnstile>{m} [ \<tau>' ; \<L> , Tail ] : \<tau> ; f \<stileturn> \<Delta>"
+    and compat: "\<Gamma> \<leftrightarrow> \<Sigma>"
+    by auto
+
+  (* Why does this need to be split into so many steps... *)
+  have "\<Gamma> \<turnstile>{m} [ \<tau>' ; \<L> , Tail ] : \<tau> ; f \<stileturn> \<Delta> \<Longrightarrow> \<exists>\<Delta>'. (\<Gamma> \<turnstile>{m} \<L> : \<tau>' ; f \<stileturn> \<Delta>') \<and> (\<exists>q. (\<Delta>' \<turnstile>{m} Tail : (q, table [] \<tau>') ; f \<stileturn> \<Delta>))"
+    apply (erule loc_type.cases)
+    by auto
+  from this and typed have "\<exists>\<Delta>'. (\<Gamma> \<turnstile>{m} \<L> : \<tau>' ; f \<stileturn> \<Delta>') \<and> (\<exists>q. (\<Delta>' \<turnstile>{m} Tail : (q, table [] \<tau>') ; f \<stileturn> \<Delta>))" 
+    by auto
+  then obtain \<Delta>' and q 
+    where loc_type_env: "\<Gamma> \<turnstile>{m} \<L> : \<tau>' ; f \<stileturn> \<Delta>'" 
+    and   tail_type_env: "\<Delta>' \<turnstile>{m} Tail : (q, table [] \<tau>') ; f \<stileturn> \<Delta>" by auto
+
+  from compat and induct and loc_type_env have "\<Delta>' \<leftrightarrow> \<Sigma>'" by auto
+  from this and induct and tail_type_env have "\<Delta> \<leftrightarrow> \<Sigma>'" by auto
+
+  then show ?case
+next
+  case (EConsListTailCongr \<L> \<Sigma> Tail \<Sigma>' Tail' \<tau>)
+  then show ?case sorry
+qed *)
+
+lemma gen_loc:
+  fixes m :: "(nat, 'a) map"
+  assumes is_fin: "finite (dom m)"
+  obtains "l" where "l \<notin> dom m"
+  using ex_new_if_finite is_fin by auto
+
+lemma located_env_compat:
+  fixes "\<Gamma>" and "\<L>" and "\<tau>" and "\<Delta>"
+  assumes "\<Gamma> \<turnstile>{m} \<L> : \<tau> ; f \<stileturn> \<Delta>"
+      and "\<Gamma> \<leftrightarrow> \<Sigma>"
+      and "located \<L>"
+    shows "\<Delta> \<leftrightarrow> \<Sigma>"
+  using assms
+proof(induction arbitrary: \<Sigma>)
   case (Nat \<Gamma> n f)
-  then have env_compat: "\<Gamma> \<leftrightarrow> (\<mu>, \<rho>)" 
-        and has_loc: "l \<notin> dom \<rho>" by auto
-  show ?case
-  proof(rule disjI2,
-        rule exI[where x = "\<mu>"], 
-        rule exI[where x = "\<rho>(l \<mapsto> (natural, Num n))"], 
-        rule exI[where x = "S (Loc (l, Amount n))"],
-        rule conjI)
-    from env_compat show "\<Gamma> \<leftrightarrow> (\<mu>, \<rho>(l \<mapsto> (natural, Num n)))" by auto
-    from has_loc show " < (\<mu>, \<rho>) , N n > \<rightarrow> < (\<mu>, \<rho>(l \<mapsto> (natural, Num n))) , S (Loc (l, Amount n)) >"
-      by (rule ENat)
-  qed
+  then show ?case by simp
 next
   case (Bool \<Gamma> b f)
-  then have env_compat: "\<Gamma> \<leftrightarrow> (\<mu>, \<rho>)" 
-        and has_loc: "l \<notin> dom \<rho>" by auto
-  show ?case
-  proof(rule disjI2,
-        rule exI[where x = "\<mu>"], 
-        rule exI[where x = "\<rho>(l \<mapsto> (boolean, Bool b))"], 
-        rule exI[where x = "S (Loc (l, SLoc l))"],
-        rule conjI)
-    from env_compat show "\<Gamma> \<leftrightarrow> (\<mu>, \<rho>(l \<mapsto> (boolean, Bool b)))" by auto
-    from has_loc show " < (\<mu>, \<rho>) , B b > \<rightarrow> < (\<mu>, \<rho>(l \<mapsto> (boolean, Bool b))) , S (Loc (l, SLoc l)) >"
-      by (rule EBool)
+  then show ?case by simp
+next
+  case (Var \<Gamma> x \<tau> m f)
+  then show ?case 
+  proof(cases x)
+    case (V x1)
+    then show ?thesis using Var.prems by simp
+  next
+    case (Loc x2)
+    then show ?thesis using Var.prems
+      by (cases \<Sigma>, simp add: domIff var_dom_def)+
   qed
+next
+  case (VarDef x \<Gamma> t f)
+  then show ?case by simp 
+next
+  case (EmptyList \<Gamma> \<tau> f)
+  then show ?case by simp
+next
+  case (ConsList \<Gamma> \<L> \<tau> f \<Delta> Tail q \<Xi>)
+  then show ?case by simp 
+qed
+
+lemma locator_progress:
+  fixes "\<Gamma>" and "\<L>" and "\<tau>" and "\<Delta>"
+  assumes "\<Gamma> \<turnstile>{m} \<L> : \<tau> ; f \<stileturn> \<Delta>"
+      and "\<Gamma> \<leftrightarrow> (\<mu>, \<rho>)"
+      and "finite (dom \<rho>)"
+  shows "located \<L> \<or> (\<exists>\<mu>' \<rho>' \<L>'. <(\<mu>, \<rho>), \<L>> \<rightarrow> <(\<mu>', \<rho>'), \<L>'>)"
+(* Premise was too strong, combined elements of progress and preservation...TODO: take some of this
+    shows "(located \<L> \<and> (\<Delta> \<leftrightarrow> (\<mu>, \<rho>)) \<and> finite (dom \<rho>))
+           \<or> (\<exists>\<mu>' \<rho>' \<L>'. (\<Delta> \<leftrightarrow> (\<mu>', \<rho>')) \<and> finite (dom \<rho>') \<and> < (\<mu>, \<rho>), \<L> > \<rightarrow> < (\<mu>', \<rho>'), \<L>' >)" *)
+  using assms
+proof(induction arbitrary: \<mu> \<rho> m rule: loc_type.induct)
+  case (Nat \<Gamma> n f)
+  then show ?case by (meson ENat gen_loc)
+next
+  case (Bool \<Gamma> b f)
+  then show ?case by (meson EBool gen_loc)
 next
   case (Var \<Gamma> x \<tau> m f)
   then have env_compat: "\<Gamma> \<leftrightarrow> (\<mu>, \<rho>)"
@@ -109,41 +218,97 @@ next
     have "x1 \<in> dom \<mu>" and eq: "x = V x1" by (auto simp: var_dom_def)
     then obtain k where in_lookup: "\<mu> x1 = Some k" by auto
     show ?thesis
-    proof(rule disjI2,
-          rule exI[where x = "\<mu>"],
-          rule exI[where x = "\<rho>"],
-          rule exI[where x = "S (Loc k)"],
-          rule conjI)
-      from env_compat and x_in_env show "\<Gamma>(x \<mapsto> f(\<tau>)) \<leftrightarrow> (\<mu>, \<rho>)" by (auto simp: var_dom_def)
-      from in_lookup and eq show "< (\<mu>, \<rho>) , S x > \<rightarrow> < (\<mu>, \<rho>) , S (Loc k) >" 
-        apply auto
-        by (rule EVar, auto)
+    proof(rule disjI2, (rule exI)+)
+      from in_lookup and eq show "< (\<mu>, \<rho>) , S x > \<rightarrow> < (\<mu>, \<rho>) , S (Loc k) >"
+        by (simp add: EVar) 
     qed
   next
     case (Loc x2)
-    then have eq: "x = Loc x2" by auto
-    show ?thesis
-    proof(rule disjI1)
-      from eq show "located (S x)" by (auto simp: located_def)
-    qed
+    then show ?thesis by simp
   qed
 next
   case (VarDef x \<Gamma> t f)
   then have env_compat: "\<Gamma> \<leftrightarrow> (\<mu>, \<rho>)" 
-        and has_loc: "l \<notin> dom \<rho>"
+        and "finite (dom \<rho>)"
         and not_in_lookup: "x \<notin> dom \<mu>" by (auto simp: var_dom_def)
+  then obtain l where has_loc: "l \<notin> dom \<rho>" using gen_loc by blast
   show ?case
-  proof(rule disjI2,
-        rule exI[where x = "\<mu>(x \<mapsto> (l, SLoc l))"],
-        rule exI[where x = "\<rho>(l \<mapsto> (t, emptyVal t))"],
-        rule exI[where x = "S (Loc (l, SLoc l))"],
-        rule conjI)
-    from env_compat show "(\<Gamma>(V x \<mapsto> f (empty, t))) \<leftrightarrow> (\<mu>(x \<mapsto> (l, SLoc l)), \<rho>(l \<mapsto> (t, emptyVal t)))"
-      by (auto simp: var_dom_def)
+  proof(rule disjI2, (rule exI)+)
     from not_in_lookup and has_loc
     show "< (\<mu>, \<rho>) , var x : t > \<rightarrow> < (\<mu>(x \<mapsto> (l, SLoc l)), \<rho>(l \<mapsto> (t, emptyVal t))) , S (Loc (l, SLoc l)) >"
       by (rule EVarDef)
   qed
+next
+  case (EmptyList \<Gamma> \<tau> f)
+  then show ?case by simp
+next
+  case (ConsList \<Gamma> \<L> \<tau> f \<Delta> Tail q \<Xi>)
+  then have env_compat: "\<Gamma> \<leftrightarrow> (\<mu>, \<rho>)" 
+        and loc_typed: "\<Gamma> \<turnstile>{s} \<L> : \<tau> ; f \<stileturn> \<Delta>"
+        and tail_typed: "\<Delta> \<turnstile>{s} Tail : (q, table [] \<tau>) ; f \<stileturn> \<Xi>"
+        and loc_induct: "located \<L> 
+                         \<or> (\<exists>\<mu>' \<rho>' \<L>''. <(\<mu>, \<rho>) , \<L>> \<rightarrow> <(\<mu>', \<rho>') , \<L>''>)"
+        and tail_induct: "\<And>\<mu> \<rho>. \<lbrakk>\<Delta> \<leftrightarrow> (\<mu>, \<rho>); finite (dom \<rho>)\<rbrakk>
+            \<Longrightarrow> located Tail
+              \<or> (\<exists>\<mu>' \<rho>' Tail'. < (\<mu>, \<rho>) , Tail > \<rightarrow> < (\<mu>', \<rho>') , Tail' >)"
+    by auto
+   
+  show ?case
+  proof(cases "located \<L>")
+    case True
+    then have loc_l: "located \<L>" 
+          and is_fin: "finite (dom \<rho>)" using ConsList.prems by auto
+    then show ?thesis 
+    proof(cases "located Tail")
+      case True
+      from this and loc_l show ?thesis by simp
+    next
+      case False
+      from loc_typed and env_compat and loc_l have "\<Delta> \<leftrightarrow> (\<mu>, \<rho>)" using located_env_compat
+        by blast
+      then have "\<exists>\<mu>' \<rho>' Tail'. < (\<mu>, \<rho>) , Tail > \<rightarrow> < (\<mu>', \<rho>') , Tail' >"
+        using tail_induct ConsList.prems(2) False by blast
+      then show ?thesis
+        using EConsListTailCongr loc_l by blast
+    qed
+  next
+    case False
+    then have "\<exists>\<mu>' \<rho>' \<L>'. < (\<mu>, \<rho>) , \<L> > \<rightarrow> < (\<mu>', \<rho>') , \<L>' >" using loc_induct by blast
+    then show ?thesis using EConsListHeadCongr by blast
+  qed
+qed
+
+fun finite_store :: "Store \<Rightarrow> bool" where
+  "finite_store (\<mu>, \<rho>) = (finite (dom \<mu>) \<and> finite (dom \<rho>))"
+
+lemma locator_preservation:
+  fixes "\<Sigma>" and "\<L>" and "\<Sigma>'" and "\<L>'"
+  assumes "<\<Sigma>, \<L>> \<rightarrow> <\<Sigma>', \<L>'>"
+      and "\<Gamma> \<turnstile>{s} \<L> : \<tau> ; (\<lambda>(_, t'). (empty, t')) \<stileturn> \<Delta>"
+      and "\<Gamma> \<leftrightarrow> \<Sigma>"
+      and "finite_store \<Sigma>"
+    shows "finite_store \<Sigma>' 
+      \<and> (\<exists>\<Gamma>' \<Delta>'. (\<Gamma>' \<leftrightarrow> \<Sigma>') \<and> (\<Gamma>' \<turnstile>{s} \<L>' : \<tau> ; (\<lambda>(_, t'). (empty, t')) \<stileturn> \<Delta>'))"
+(*TODO: We may need some compatibility condition between \<Gamma> and \<Gamma>' and \<Delta> and \<Delta>' *)
+  using assms
+proof(induction arbitrary: \<Gamma> \<tau> \<Delta>)
+case (ENat l \<rho> \<mu> n)
+  then show ?case
+next
+  case (EBool l \<rho> \<mu> b)
+  then show ?case sorry
+next
+  case (EVar \<mu> x l \<rho>)
+  then show ?case sorry
+next
+  case (EVarDef x \<mu> l \<rho> t)
+  then show ?case sorry
+next
+  case (EConsListHeadCongr \<Sigma> \<L> \<Sigma>' \<L>' \<tau> Tail)
+  then show ?case sorry
+next
+  case (EConsListTailCongr \<L> \<Sigma> Tail \<Sigma>' Tail' \<tau>)
+  then show ?case sorry
 qed
 
 end
